%
% Copyright Â© 2018 Peeter Joot.  All Rights Reserved.
% Licenced as described in the file LICENSE under the root directory of this GIT repository.
%
%\paragraph{Useful identities.}

\section{Review of old material.}

\begin{itemize}
\item Gaussian
\begin{dmath}\label{eqn:usefulFormulas:20}
\int_{-\infty}^\infty e^{a x^2} dx = \sqrt{\frac{-\pi}{a}}.
\end{dmath}
Here \( a \) may be real or imaginary, but must be less than 0 if real.
\item Our Fourier transform sign and \( \pi \) placement convention (\( 2 \pi\)'s with momentum elements and negative exponential sign for the inverse transform)
\begin{dmath}\label{eqn:usefulFormulas:40}
\begin{aligned}
f(x) &= \int \frac{d^n k}{(2 \pi)^n} f(k) e^{i k \cdot x} \\
f(k) &= \int d^n x f(x) e^{-i k \cdot x}.
\end{aligned}
\end{dmath}
\item Delta function representation.

Setting \( f(x) = \delta^n(x) \) implies \( f(k) = 1 \) and so
\begin{dmath}\label{eqn:usefulFormulas:60}
\delta(x) = \int \frac{d^n k}{(2 \pi)^n} e^{i k \cdot x}.
\end{dmath}

\item Correct sign for the commutator
\begin{dmath}\label{eqn:usefulFormulas:80}
\antisymmetric{x_r}{p_s} = i \delta_{rs}.
\end{dmath}
\item Hamilton's equations
\begin{dmath}\label{eqn:usefulFormulas:100}
\begin{aligned}
-dH &= d(\LL - p \dot{q}) = \PD{q}{\LL} dq + \cancel{\PD{\dot{q}}{\LL} d\dot{q}} + \PD{t}{\LL} dt - dp \dot{q} - \cancel{p d\dot{q}} \\
dH &=
\PD{q}{H} dq
+
\PD{p}{H} dp
+
\PD{t}{H} dt,
\end{aligned}
\end{dmath}
so
\begin{equation}\label{eqn:usefulFormulas:120}
\PD{q}{H} = -\dot{p},\qquad
\PD{p}{H} = \dot{q},\qquad
\PD{t}{H} = -\PD{t}{\LL}.
\end{equation}
\item Matrix element for the momentum and position operators
\begin{dmath}\label{eqn:usefulFormulas:140}
\begin{aligned}
\bra{x} P \ket{x'} &= -i \delta(x- x') \frac{d}{dx} \\
\bra{p} X \ket{p'} &= i \delta(p- p') \frac{d}{dp}.
\end{aligned}
\end{dmath}
\item Eigenstates
\begin{dmath}\label{eqn:usefulFormulas:160}
\begin{aligned}
p \braket{x}{p}
&= \bra{x} P \ket{p} \\
&= \int dx' \bra{x} P \ket{x'} \braket{x'}{p} \\
&= \int dx' (-i) \delta(x - x') \frac{d}{dx} \braket{x'}{p} \\
&= -i \frac{d}{dx} \braket{x}{p},
\end{aligned}
\end{dmath}
so
\begin{dmath}\label{eqn:usefulFormulas:180}
\braket{x}{p} \propto e^{i p x}.
\end{dmath}
Normalized over all space in \( d \) dimensions
\begin{dmath}\label{eqn:usefulFormulas:200}
\braket{x}{p} = \frac{e^{i p \cdot x}}{(2 \pi)^{d/2}}.
\end{dmath}
\item Time evolution in the Heisenberg picture
\begin{dmath}\label{eqn:usefulFormulas:220}
\ddt{O} = i \antisymmetric{H}{O}.
\end{dmath}
\item Commutators of powers of position and momentum operators
\begin{dmath}\label{eqn:usefulFormulas:240}
\begin{aligned}
\antisymmetric{\hatq^n}{\hatp} &= n i \hatq^{n-1} \\
\antisymmetric{\hatp^n}{\hatq} &= -n i \hatp^{n-1}.
\end{aligned}
\end{dmath}
More generally, for any function with a power series representation \( F(x) = \sum_{k = 0}^\infty a_k x^k \), we have
\begin{dmath}\label{eqn:usefulFormulas:260}
\begin{aligned}
\antisymmetric{F(\hatq)}{\hatp} &= i \frac{dF}{d\hatq} \\
\antisymmetric{F(\hatp)}{\hatq} &= -i \frac{dF}{d\hatp}.
\end{aligned}
\end{dmath}
\item Pauli matrices
\begin{equation}\label{eqn:usefulFormulas:280}
\sigma^1 = \PauliX, \quad
\sigma^2 = \PauliY, \quad
\sigma^3 = \PauliZ.
\end{equation}
\begin{dmath}\label{eqn:usefulFormulas:300}
\antisymmetric{\sigma^a}{\sigma^b} = 2 i \epsilon^{a b c} \sigma^c.
\end{dmath}
\item Euler-Lagrange equations
\begin{dmath}\label{eqn:usefulFormulas:320}
\PD{\phi}{\LL} - \partial_\mu \PD{(\partial_\mu \phi)}{\LL} = 0.
\end{dmath}
\item Lorentz transform identities
\begin{dmath}\label{eqn:usefulFormulas:340}
g_{\nu\rho}
=
g_{\mu \kappa}
{\Lambda^\mu}_\nu
{\Lambda^\kappa}_\rho.
\end{dmath}
\item Noether's first theorem.  Given \( \delta \LL = \partial_\mu J^\mu \),
\begin{dmath}\label{eqn:usefulFormulas:480}
j^\mu =
\frac{\delta \LL}{\delta(\partial_\mu \phi)} \delta \phi  - J^\mu,
\end{dmath}
satisfies \( \partial_\mu j^\mu = 0 \).
\item Energy momentum tensor
\begin{dmath}\label{eqn:usefulFormulas:500}
T^{\mu\nu} = \partial^\mu \phi \partial^\nu \phi - g^{\mu\nu} \LL.
\end{dmath}
\item Translation operator
\begin{dmath}\label{eqn:usefulFormulas:520}
\hatU(\Ba) = e^{i \Ba \cdot \hat{\BP}},
\end{dmath}
\begin{dmath}\label{eqn:usefulFormulas:540}
\bra{\Bx} \hatU(\Ba) = \bra{\Bx + \Ba}
\end{dmath}
\item Baker-Campbell-Hausdorff theorem \cref{thm:qftLecture8:580}.
\begin{dmath}\label{eqn:usefulFormulas:560}
e^{B} A e^{-B} = \sum_{n = 0}^\infty \inv{n!} \antisymmetric{B \cdots}{\antisymmetric{B}{A}}.
\end{dmath}
\end{itemize}

\section{Useful results from new material.}

\begin{itemize}
\item Hamiltonian for a massive scalar field
\begin{dmath}\label{eqn:usefulFormulas:360}
H
= \int d^3 x \lr{ \inv{2} (\pi(\Bx, t))^2 + \inv{2} (\spacegrad \phi(\Bx, t))^2 + \frac{m}{2} (\phi(\Bx, t))^2 }
\end{dmath}
\begin{dmath}\label{eqn:usefulFormulas:380}
\normalorder{H}
= \int \frac{d^3 p}{(2 \pi)^3} \omega_\Bp a_\Bp^\dagger a_\Bp
\end{dmath}
\item Canonical commutator
\begin{dmath}\label{eqn:usefulFormulas:400}
\antisymmetric{\pi(\Bx, t)}{\phi(\By, t)} = -i \deltathree(\Bx - \By).
\end{dmath}
\item Creation and annhilation operation
\begin{dmath}\label{eqn:usefulFormulas:420}
\antisymmetric
{a_\Bq}
{a^\dagger_\Bp}
=
(2 \pi)^3
\deltathree(\Bp - \Bq).
\end{dmath}
\begin{dmath}\label{eqn:usefulFormulas:440}
\phi(\Bx, t)
=
\int \frac{d^3 p}{(2\pi)^3} \inv{\sqrt{2 \omega_\Bp}} e^{i \Bp \cdot \Bx}
\lr{
   e^{-i \omega_\Bp t} a_\Bp
   +
   e^{i \omega_\Bp t} a_{-\Bp}^\dagger
}
\end{dmath}
\begin{dmath}\label{eqn:usefulFormulas:460}
\pi(\Bx, t)
=
\int \frac{d^3 q}{(2\pi)^3}
\frac{i \omega_\Bq }{ \sqrt{2 \omega_\Bq}}
e^{i \Bq \cdot \Bx}
\lr{
   -e^{-i \omega_\Bq t} a_\Bq
   +
   e^{i \omega_\Bq t} a_{-\Bq}^\dagger
}.
\end{dmath}
\item Relativisitic normalization and transformation of momentum state
\begin{dmath}\label{eqn:usefulFormulas:580}
\sqrt{2 \omega_{ \Bp}} \hata^\dagger_{ \Bp} \ket{0} = \ket{\Bp},
\end{dmath}
\begin{dmath}\label{eqn:usefulFormulas:600}
\hatU(\Lambda) \ket{\Bp} = \ket{\Lambda \Bp}.
\end{dmath}
\item Plus and minus operators
\begin{dmath}\label{eqn:usefulFormulas:620}
\begin{aligned}
\phihat_{-}(x) &=
\int \frac{d^3 p}{(2 \pi)^3 \sqrt{2 \omega_\Bp}}
\evalbar{
e^{-i p \cdot x} }{p^0 = \omega_\Bp} \hata_\Bp \\
\phihat_{+}(x) &=
\int \frac{d^3 p}{(2 \pi)^3 \sqrt{2 \omega_\Bp}}
\evalbar{
e^{i p \cdot x} }{p^0 = \omega_\Bp} \hata^\dagger_\Bp.
\end{aligned}
\end{dmath}
\item Wightman function
\begin{equation}\label{eqn:usefulFormulas:640}
D(x)
= \antisymmetric{\phihat_{-}(x)}{\phihat_{+}(0)}
=
\int \frac{d^3 p}{(2 \pi)^3 2 \omega_\Bp}
\evalbar{ e^{-i p \cdot x} }{p^0 = \omega_\Bp}.
\end{equation}
\item Contractions with momentum states
\begin{dmath}\label{eqn:usefulFormulas:660}
\begin{aligned}
\contraction{}{\phi}{{}_I(x)}{a}
\phi_I(x) a^\dagger_{\Bp}
&= e^{-i p \cdot x} \\
\contraction{}{a}{{}_\Bp}{\phi}
a_\Bp \phi_I(x)
&= e^{i p \cdot x}.
\end{aligned}
\end{dmath}
\end{itemize}
